YLM: functions for installation of long term keys of principals and auth server

yahalom/YLM.Debug.fst
@@ -1,1 +1,53 @@
 module YLM.Debug
+
+
+open SecrecyLabels
+open CryptoEffect
+open CryptoLib
+open GlobalRuntimeLib
+open LabeledCryptoAPI
+open LabeledRuntimeAPI
+open LabeledPKI
+open AttackerAPI
+open SecurityLemmas
+open YLM.Sessions
+open YLM.Protocol
+
+
+val benign_attacker:
+  unit ->
+  LCrypto unit (pki ylm_preds)
+  (requires fun _ -> True)
+  (ensures fun _ _ _ -> True)
+
+#set-options "--z3rlimit 200 --max_fuel 4 --max_ifuel 2"
+let benign_attacker () =
+  let a:principal = "alice" in
+  let b:principal = "bob" in
+  let srv:principal = "server" in
+
+  let ((|t_kas,k_as|), kas_idx) = new_lt_key_session a srv in
+  let ((|t_kbs,k_bs|), kbs_idx) = new_lt_key_session b srv in
+  install_lt_key_at_auth_server #t_kas srv a k_as;
+  install_lt_key_at_auth_server #t_kbs srv b k_bs;
+  ()
+
+let benign () : LCrypto unit (pki ylm_preds)
+  (requires (fun _ -> True)) (ensures (fun _ _ _ -> True))
+= print_string "start\n";
+  let t0 = get () in
+  let x = benign_attacker () in
+  print_trace ()
+
+let main =
+  IO.print_string "======================\n";
+  IO.print_string "Yahalom               \n";
+  IO.print_string "======================\n";
+  let t0 = Seq.empty in
+  IO.print_string "Starting Benign Attacker:\n";
+  assume(valid_trace (pki ylm_preds) t0);
+  let r,t1 = (reify (benign ()) t0) in
+  (match r with
+  | Error s -> IO.print_string ("ERROR: "^s^"\n")
+  | Success _ -> IO.print_string "PROTOCOL RUN: Successful execution of Yahalom protocol.\n");
+  IO.print_string "Finished Benign Attacker:\n"
