yahalom/YLM.Protocol.fsti
@@ -1,1 +1,30 @@
 module YLM.Protocol
+
+
+open SecrecyLabels
+open CryptoEffect
+open CryptoLib
+open GlobalRuntimeLib
+open YLM.Messages
+open YLM.Sessions
+open LabeledCryptoAPI
+open LabeledRuntimeAPI
+open LabeledPKI
+
+
+val new_lt_key_session:
+  p:principal ->
+  server:principal ->
+  LCrypto ((i:timestamp & k_ps:lt_key i p server) * sess_idx:nat) (pki ylm_preds)
+  (requires (fun t0 -> True))
+  (ensures (fun t0 ((|i,k_ps|), si) t1 ->
+    i == trace_len t0 /\ trace_len t1 == trace_len t0 + 2))
+
+val install_lt_key_at_auth_server:
+  #i:nat ->
+  server:principal ->
+  p:principal ->
+  k_ps:lt_key i p server ->
+  LCrypto unit (pki ylm_preds)
+  (requires (fun t0 -> i < trace_len t0))
+  (ensures (fun t0 _ t1 -> trace_len t1 == trace_len t0 + 1))
